Sync theories with branch 'main'

theories/coq/ElaborationSoundness.v
@@ -30,7 +30,7 @@ Proof with eauto using ttyp_trans_wf.
   introv HU. induction* G.
   simpl... destruct a... econstructor...
   inverts~ HU.
-  Qed.
+Qed.
 
 Open Scope list.
 
@@ -66,7 +66,7 @@ intuition eauto using target_typing_wf_1, target_typing_wf_2,
   introv HC HTa Eqa Eqa' HTb Eqb Eqb'. gen E t1 t2 t B T1 T2.
   indTypSize (size_typ A1 + size_typ A2). inverts HC.
   - exists. splits;
-    try rewrite ttyp_trans_ord_top; try rewrite* <- check_toplike_sound_complete...
+      try rewrite ttyp_trans_ord_top; try rewrite* <- check_toplike_sound_complete...
   - forwards (?&?&?): ST_concat Eqa' Eqb'.
     applys* concat_source_intersection...
     1-4: auto... intuition eauto using target_typing_wf_typ.
@@ -212,14 +212,14 @@ intuition eauto using target_typing_wf_1, target_typing_wf_2,
     Unshelve. all: eauto.
 Qed.
 
-Lemma check_toplike_false : forall B,
+Lemma check_toplike_false_2 : forall B,
     ~ toplike B -> check_toplike B = false.
 Proof.
   introv TL. remember (check_toplike B). destruct* b.
   exfalso. applys TL. rewrite* check_toplike_sound_complete.
 Qed.
 
-#[local] Hint Resolve check_toplike_false : core.
+#[local] Hint Resolve check_toplike_false_2 : core.
 
 Lemma split_toplike : forall A B C,
     spl A B C -> toplike B -> toplike C -> toplike A.
@@ -235,7 +235,7 @@ Proof.
   introv HC HT HTA. applys HT. clear HT. gen t1 t2.
   indTypSize (size_typ A + size_typ B).
   inverts HC. 1-7: inverts~ HTA.
-  - pick fresh x; try lets (?&?): H1 x; intuition eauto.
+  - pick fresh x; try lets (?&?&?): H1 x. intuition eauto.
     forwards*: IH H4. elia.
   - forwards*: IH H1. elia.
   - forwards*: IH H0. elia.
@@ -243,6 +243,609 @@ Proof.
   - forwards*: IH H0. elia. forwards*: IH H1. elia.
     eauto using split_toplike.
 Qed.
+
+(** *********************************** *)
+#[local] Hint Constructors esub : core.
+
+Lemma esub_is_term_erased_cosub_1 : forall A B,
+    (exists t1 t2, cosub t1 A B t2) -> esub A B.
+Proof with elia.
+  intros. destruct_conj. gen x x0.
+  indTypSize (size_typ A + size_typ B).
+  destruct* H.
+  + { pick fresh x.
+      forwards* (?&Hx1&Hx2): H1 x.
+      forwards: IH Hx1... forwards: IH Hx2... applys* ES_Arrow. }
+  + { forwards: IH H1... eauto. }
+  + { forwards: IH H0... eauto. }
+  + { forwards: IH H0... eauto. }
+  + { forwards: IH H0... forwards: IH H1... eauto. }
+Qed.
+
+Lemma comerge_lc_texp : forall t1 A B t2 C t3,
+    comerge t1 A B t2 C t3 -> lc_texp t3.
+Proof with elia.
+  introv HC. gen t1 t2 t3 A B.
+  indTypSize (size_typ C).
+  destruct* HC.
+  - { econstructor. pick fresh x. forwards* Hx: H1 x.
+      forwards: IH Hx...
+      applys* lc_texp_abs_exists. eauto. }
+  - { econstructor. pick fresh x. forwards* Hx: H2 x.
+      forwards: IH Hx...
+      applys* lc_texp_abs_exists. eauto. }
+  - { econstructor. pick fresh x. forwards* Hx: H2 x.
+      forwards: IH Hx...
+      applys* lc_texp_abs_exists. eauto. }
+  - repeat econstructor; forwards~: IH HC...
+  - repeat econstructor; forwards~: IH HC...
+  - repeat econstructor; forwards~: IH HC...
+Qed.
+
+Lemma comerge_lc_texp_1 : forall t1 A t2 B C t3,
+    comerge t1 A B t2 C t3 -> lc_texp t1.
+Proof with elia.
+  introv HC. gen t1 t2 t3 A C.
+  indTypSize (size_typ B). inverts* HC.
+  - pick fresh x. instantiate_cofinites_with x.
+    forwards: IH H1... inverts H2. inverts ~H5.
+  - pick fresh x. instantiate_cofinites_with x.
+    forwards: IH H2... inverts H3. inverts ~H6.
+  - pick fresh x. instantiate_cofinites_with x.
+    forwards: IH H1... inverts~ H2.
+  - forwards: IH H2... inverts~ H3.
+Qed.
+
+Lemma comerge_lc_texp_2 : forall t1 A t2 B C t3,
+    comerge t1 A B t2 C t3 -> lc_texp t2.
+Proof with elia.
+  introv HC. gen t1 t2 t3 A C.
+  indTypSize (size_typ B). inverts* HC.
+  - pick fresh x. instantiate_cofinites_with x.
+    forwards: IH H1... inverts H2. inverts ~H5.
+  - pick fresh x. instantiate_cofinites_with x.
+    forwards: IH H2... inverts H3. inverts ~H6.
+  - pick fresh x. instantiate_cofinites_with x.
+    forwards: IH H1... inverts~ H2.
+  - forwards: IH H2... inverts~ H3.
+Qed.
+
+
+Lemma cosub_lc_texp : forall A B t1 t2,
+    cosub t1 A B t2 -> lc_texp t2.
+Proof with elia.
+  introv HC. gen t1 t2.
+  indTypSize (size_typ A + size_typ B).
+  destruct* HC.
+  2: { econstructor. pick fresh x. forwards* (?& Hx): H1 x.
+       forwards: IH Hx...
+       applys* lc_texp_abs_exists. eauto. }
+  all: repeat econstructor.
+  all: try forwards~: IH HC...
+  eauto using comerge_lc_texp.
+Qed.
+
+Lemma toplike_dec : forall A, { toplike A } + { ~ toplike A }.
+Proof.
+  introv.
+  remember (check_toplike A) as P. destruct P.
+  - left*. applys* check_toplike_sound_complete.
+  - right*. lets*: check_toplike_false A.
+Qed.
+
+
+Notation "[ z ~~> u ] t" := (subst_texp u z t) (at level 0).
+Notation "[ x ~=> y ] t" := (subst_texp (texp_var_f y) x t) (at level 0).
+Notation "t ^-^ u"       := (open_texp_wrt_texp t u) (at level 67).
+Notation "t -^ x"        := (open_texp_wrt_texp t (texp_var_f x))(at level 67).
+
+#[local] Hint Resolve subst_texp_lc_texp comerge_lc_texp comerge_lc_texp_1 comerge_lc_texp_2 : core.
+
+Ltac simp_eq Eq :=
+  let Heq := fresh "Heq" in
+  assert (Heq: Eq) by default_simp ; rewrite Heq.
+
+Ltac simp_eq_in Eq H :=
+  let Heq := fresh "Heq" in
+  assert (Heq: Eq) by default_simp ; rewrite Heq in H.
+
+Lemma comerge_rename : forall t1 t2 t3 A B C x y,
+    (* y `notin` ((fv_texp t1) `union` (fv_texp t2)) -> *)
+    comerge t1 B A t2 C t3 ->
+    comerge ([ x ~=> y ] t1) B A ([ x ~=> y ] t2) C ([ x ~=> y ] t3).
+Proof with try solve_notin.
+  introv HC. gen x y.
+  induction HC; intros.
+  1-2: default_simp.
+  5: {
+    applys~ M_RcdL.
+    forwards: IHHC x y...  }
+  5: {
+    applys~ M_RcdR.
+    forwards: IHHC x y...  }
+  4: {
+    simp_eq ([x ~=> y] (texp_cons (|| typ_rcd l A ||) t texp_nil) = (texp_cons (|| typ_rcd l A ||) ([x ~=> y] t) texp_nil) ).
+    applys~ M_Rcd.
+    forwards: IHHC x y...
+  }
+  3: {
+    remember (|| typ_arrow A B1 ||) as l1.
+    remember (|| typ_arrow A B2 ||) as l2.
+    remember (|| typ_arrow A B ||) as l.
+    simp_eq ([x ~=> y] (texp_cons l (texp_abs t) texp_nil) =  texp_cons l (texp_abs ([x ~=> y] t)) texp_nil).
+    rewrite Heql.
+    applys* M_ArrowR ((L \u {{x}} \u {{y}})).
+    intros z Fr_z.
+    forwards: H3 z x y...
+    rewrite~ subst_texp_open_texp_wrt_texp in H4.
+    simp_eq_in ([x ~=> y] (texp_var_f z) = texp_var_f z) H4.
+    rewrite <- Heql2. case_if*. { subst. solve_notin. }
+  }
+  2: {
+    remember (|| typ_arrow A B1 ||) as l1.
+    remember (|| typ_arrow A B2 ||) as l2.
+    remember (|| typ_arrow A B ||) as l.
+    simp_eq ([x ~=> y] (texp_cons l (texp_abs t) texp_nil) =  texp_cons l (texp_abs ([x ~=> y] t)) texp_nil).
+    rewrite Heql.
+    applys* M_ArrowL ((L \u {{x}} \u {{y}})).
+    intros z Fr_z.
+    forwards: H3 z x y...
+    rewrite~ subst_texp_open_texp_wrt_texp in H4.
+    simp_eq_in ([x ~=> y] (texp_var_f z) = texp_var_f z) H4.
+    rewrite <- Heql1. case_if*. { subst. solve_notin. }
+  }
+  1: {
+    remember (|| typ_arrow A B1 ||) as l1.
+    remember (|| typ_arrow A B2 ||) as l2.
+    remember (|| typ_arrow A B ||) as l.
+    simp_eq ([x ~=> y] (texp_cons l (texp_abs t) texp_nil) =  texp_cons l (texp_abs ([x ~=> y] t)) texp_nil).
+    rewrite Heql.
+    applys* M_Arrow ((L \u {{x}} \u {{y}})).
+    intros z Fr_z.
+    forwards: H2 z x y...
+    rewrite~ subst_texp_open_texp_wrt_texp in H3.
+    simp_eq_in ([x ~=> y] (texp_var_f z) = texp_var_f z) H3.
+    rewrite <- Heql1. rewrite <- Heql2. case_if*. { subst. solve_notin. }
+  }
+Qed.
+
+Lemma fv_texp_comerge : forall t1 t2 t3 A B C,
+    comerge t1 A C t2 B t3 -> (fv_texp t3) [<=] (fv_texp t1) \u (fv_texp t2).
+Proof with simpl; try fsetdec.
+  introv HC. induction* HC...
+  - instantiate_cofinites.
+    pose proof fv_texp_open_texp_wrt_texp_lower t (texp_var_f x).
+    simpl in H2...
+  - instantiate_cofinites.
+    pose proof fv_texp_open_texp_wrt_texp_lower t (texp_var_f x).
+    simpl in H3...
+  - instantiate_cofinites.
+    pose proof fv_texp_open_texp_wrt_texp_lower t (texp_var_f x).
+    simpl in H3...
+Qed.
+
+Lemma cosub_rename : forall t1 t2 A B x y,
+    (* y `notin` ((fv_texp t1) `union` (fv_texp t2)) -> *)
+    cosub t1 A B t2 ->
+    cosub ([ x ~=> y ] t1) A B ([ x ~=> y ] t2).
+Proof with elia; try solve_notin.
+  introv HC. gen x y t1 t2. indTypSize (size_typ A + size_typ B).
+  destruct* HC.
+  7: {
+    forwards: comerge_rename x y H0...
+    forwards: IH HC1... forwards: IH HC2...
+    eauto.
+  }
+  5, 6 : forwards: IH x y HC...
+  2: {
+    simp_eq ([x ~=> y] (texp_cons (|| typ_base ||) (texp_proj t (|| typ_base ||)) texp_nil) = (texp_cons (|| typ_base ||) (texp_proj ([x ~=> y] t) (|| typ_base || )) texp_nil)).
+    eauto. }
+  1: {
+    simp_eq ([x ~=> y] (texp_cons (|| B ||) (texp_fixpoint (texp_var_b 0)) texp_nil) = (texp_cons (|| B ||) (texp_fixpoint (texp_var_b 0)) texp_nil)).
+    eauto.
+  }
+  2: { (* rcd *)
+    forwards: IH HC...
+    simp_eq_in ( [x ~=> y] (texp_proj t (|| typ_rcd l A ||)) =  (texp_proj ([x ~=> y] t) (|| typ_rcd l A ||)) ) H1.
+    simp_eq ( [x ~=> y] (texp_cons (|| typ_rcd l B ||) t2 texp_nil) = (texp_cons (|| typ_rcd l B ||) ([x ~=> y] t2) texp_nil)) .
+    eauto.
+  }
+  1: { (* arrow *)
+    simp_eq ( [x ~=> y] (texp_cons (|| typ_arrow B1 B2 ||) (texp_abs t2) texp_nil) = (texp_cons (|| typ_arrow B1 B2 ||) (texp_abs [x ~=> y] t2) texp_nil) ).
+    applys~ S_Arrow (L \u {{x}}). intros z Fr.
+    remember (|| typ_arrow A1 A2 ||) as l2.
+    forwards* (?&?&?): H1 z.
+    forwards: IH x y H2...
+    simp_eq_in ([x ~=> y] (texp_var_f z) = texp_var_f z) H4.
+    forwards: IH x y H3...
+    simp_eq_in ([x ~=> y] (texp_app (texp_proj t l2) x0) = texp_app (texp_proj ([x ~=> y] t) l2) ([x ~=> y] x0)) H5.
+    exists*. split*.
+    rewrite~ subst_texp_open_texp_wrt_texp in H5.
+    simp_eq_in ([x ~=> y] (texp_var_f z) = texp_var_f z) H5.
+    eauto.
+  }
+Qed.
+
+Theorem spl_sound_to_comerge : forall A B C t u,
+    spl A B C -> lc_texp t -> lc_texp u -> exists z, comerge t B A u C z.
+Proof with try fsetdec; elia.
+  introv HS HL1 HL2. gen t u. induction HS; intros.
+  - forwards* [?|?]: toplike_dec (typ_and A B).
+  - forwards* [?|?]: toplike_dec (typ_arrow A B1);
+      forwards* [?|?]: toplike_dec (typ_arrow A B2).
+    + destruct_conj. forwards*: split_toplike (typ_arrow A B).
+    + pick fresh y.
+      remember (|| typ_arrow A B2 ||) as l1.
+      forwards* (tt&HL): IHHS texp_nil (texp_app (texp_proj u l1) (texp_var_f y)).
+      rewrite <- (open_texp_wrt_texp_close_texp_wrt_texp tt y) in HL.
+      exists. applys* M_ArrowR ((fv_texp (texp_var_f y)) `union` (fv_texp tt) `union` (fv_texp t)`union` (fv_texp u) `union` (fv_texp tt)) (close_texp_wrt_texp y tt). inverts~ t0.
+      introv Fr_x.
+      forwards* HC: comerge_rename y x HL.
+      rewrite <- Heql1.
+      rewrite~ subst_texp_open_texp_wrt_texp in HC.
+      assert (Heq: [y ~=> x] (texp_var_f y) = texp_var_f x).
+      { default_simp. }
+      rewrite Heq in HC.
+      assert (Heq': [y ~=> x] texp_nil = texp_nil).
+      { default_simp. }
+      rewrite Heq' in HC.
+      assert (Heq2: [y ~=> x] (texp_app (texp_proj u l1) (texp_var_f y)) = (texp_app (texp_proj u l1) (texp_var_f x))).
+      { default_simp. rewrite* subst_texp_fresh_eq. }
+      rewrite Heq2 in HC.
+      assert (Heq3: [y ~=> x] (close_texp_wrt_texp y tt) = (close_texp_wrt_texp y tt)). {
+        apply subst_texp_fresh_eq...
+        rewrite fv_texp_close_texp_wrt_texp. eauto.
+      }
+      rewrite Heq3 in HC. simpl in HC. now auto.
+    + pick fresh y.
+      remember (|| typ_arrow A B1 ||) as l1.
+      forwards* (tt&HL): IHHS (texp_app (texp_proj t l1) (texp_var_f y)) texp_nil .
+      rewrite <- (open_texp_wrt_texp_close_texp_wrt_texp tt y) in HL.
+      exists. applys* M_ArrowL ((fv_texp (texp_var_f y)) `union` (fv_texp tt) `union` (fv_texp t)`union` (fv_texp u) `union` (fv_texp tt)) (close_texp_wrt_texp y tt). inverts~ t0.
+      introv Fr_x.
+      forwards* HC: comerge_rename y x HL.
+      rewrite <- Heql1.
+      rewrite~ subst_texp_open_texp_wrt_texp in HC.
+      assert (Heq: [y ~=> x] (texp_var_f y) = texp_var_f x).
+      { default_simp. }
+      rewrite Heq in HC.
+      assert (Heq': [y ~=> x] texp_nil = texp_nil).
+      { default_simp. }
+      rewrite Heq' in HC.
+      assert (Heq2: [y ~=> x] (texp_app (texp_proj t l1) (texp_var_f y)) = (texp_app (texp_proj t l1) (texp_var_f x))).
+      { default_simp. rewrite* subst_texp_fresh_eq. }
+      rewrite Heq2 in HC.
+      assert (Heq3: [y ~=> x] (close_texp_wrt_texp y tt) = (close_texp_wrt_texp y tt)). {
+        apply subst_texp_fresh_eq...
+        rewrite fv_texp_close_texp_wrt_texp. eauto.
+      }
+      rewrite Heq3 in HC. simpl in HC. now auto.
+    + pick fresh y.
+      remember (|| typ_arrow A B1 ||) as l1.
+      remember (|| typ_arrow A B2 ||) as l2.
+      forwards* (tt&HL): IHHS (texp_app (texp_proj t l1) (texp_var_f y)) (texp_app (texp_proj u l2) (texp_var_f y)) .
+      rewrite <- (open_texp_wrt_texp_close_texp_wrt_texp tt y) in HL.
+      exists. applys* M_Arrow ((fv_texp (texp_var_f y)) `union` (fv_texp tt) `union` (fv_texp t)`union` (fv_texp u) `union` (fv_texp tt)) (close_texp_wrt_texp y tt).
+      introv Fr_x.
+      forwards* HC: comerge_rename y x HL.
+      rewrite <- Heql1. rewrite <- Heql2.
+      rewrite~ subst_texp_open_texp_wrt_texp in HC.
+      assert (Heq: [y ~=> x] (texp_var_f y) = texp_var_f x).
+      { default_simp. }
+      rewrite Heq in HC.
+      assert (Heq2: [y ~=> x] (texp_app (texp_proj t l1) (texp_var_f y)) = (texp_app (texp_proj t l1) (texp_var_f x))).
+      { default_simp. rewrite* subst_texp_fresh_eq. }
+      rewrite Heq2 in HC.
+      assert (Heq2': [y ~=> x] (texp_app (texp_proj u l2) (texp_var_f y)) = (texp_app (texp_proj u l2) (texp_var_f x))).
+      { default_simp. rewrite* subst_texp_fresh_eq. }
+      rewrite Heq2' in HC.
+      assert (Heq3: [y ~=> x] (close_texp_wrt_texp y tt) = (close_texp_wrt_texp y tt)). {
+        apply subst_texp_fresh_eq...
+        rewrite fv_texp_close_texp_wrt_texp. eauto.
+      }
+      rewrite Heq3 in HC. simpl in HC. now auto.
+  - forwards* [?|?]: toplike_dec (typ_rcd l B1);
+      forwards* [?|?]: toplike_dec (typ_rcd l B2).
+    + destruct_conj. forwards*: split_toplike (typ_rcd l B).
+    + remember (|| typ_rcd l B2 ||) as l2.
+      forwards~ (?&?): IHHS texp_nil (texp_proj u l2).
+      exists. applys~ M_RcdR. inverts~ t0.
+      rewrite <- Heql2. applys H.
+    + remember (|| typ_rcd l B1 ||) as l1.
+      forwards~ (?&?): IHHS (texp_proj t l1) texp_nil.
+      exists. applys~ M_RcdL. inverts~ t0.
+      rewrite <- Heql1. applys H.
+    + remember (|| typ_rcd l B1 ||) as l1.
+      remember (|| typ_rcd l B2 ||) as l2.
+      forwards~ (?&?): IHHS (texp_proj t l1) (texp_proj u l2).
+      exists. applys~ M_Rcd.
+      rewrite <- Heql1. rewrite <- Heql2. applys H.
+Qed.
+
+#[local] Hint Immediate cosub_lc_texp : core.
+Lemma esub_is_term_erased_cosub_2 : forall A B t1,
+    esub A B -> lc_texp t1 -> (exists t2, cosub t1 A B t2).
+Proof with try fsetdec; elia.
+  introv HE HC. gen t1.
+  indTypSize (size_typ A + size_typ B).
+  destruct* HE.
+  + exists. applys* S_Bot. pick fresh a. eauto.
+  + pick fresh y.
+    forwards* (tt&HC1): IH HE1 (texp_var_f y)...
+    remember (|| typ_arrow A1 A2 ||) as l1.
+    forwards* (t2'&HC2): IH HE2 (texp_app (texp_proj t1 l1) tt)...
+    rewrite <- (open_texp_wrt_texp_close_texp_wrt_texp t2' y) in HC2.
+    clear HE1 HE2 SizeInd.
+    exists.
+    applys* S_Arrow ((fv_texp (texp_var_f y)) `union` (fv_texp tt) `union` (fv_texp t1) `union` (fv_texp t2')) (close_texp_wrt_texp y t2').
+    intros x Frx. rewrite <- Heql1. exists. split.
+    * forwards*: cosub_rename y x HC1...
+      assert (Heq: [y ~=> x] (texp_var_f y) = texp_var_f x).
+      { default_simp. }
+      rewrite Heq in H1. applys H1.
+    * forwards*: cosub_rename y x HC2...
+      rewrite subst_texp_open_texp_wrt_texp in H1.
+      assert (Heq: [y ~=> x] (texp_var_f y) = texp_var_f x).
+      { default_simp. }
+      rewrite Heq in H1.
+      ** assert (Heq2: [y ~=> x] (texp_app (texp_proj t1 l1) tt) = (texp_app (texp_proj t1 l1) [y ~=> x] (tt))).
+         { default_simp. rewrite* subst_texp_fresh_eq. }
+         rewrite Heq2 in H1.
+         assert (Heq3: [y ~=> x] (close_texp_wrt_texp y t2') = (close_texp_wrt_texp y t2')). {
+           apply subst_texp_fresh_eq...
+           rewrite fv_texp_close_texp_wrt_texp. eauto.
+         }
+         rewrite Heq3 in H1. auto.
+      ** eauto.
+  + forwards (?&?): IH HE  (texp_proj t1 (|| typ_rcd l A ||))...
+    all: eauto.
+  + forwards (?&?): IH HE t1...
+    all: eauto.
+  + forwards (?&?): IH HE t1...
+    all: eauto.
+  + forwards* (?&?): IH HE1 t1...
+    forwards* (?&?): IH HE2 t1...
+    forwards* (?&?): spl_sound_to_comerge x x0 H.
+Qed.
+
+Theorem esub_is_term_erased_cosub : forall A B,
+    esub A B <-> (forall t1, lc_texp t1 -> exists t2, cosub t1 A B t2).
+Proof.
+  introv. split.
+  - intros. pose proof esub_is_term_erased_cosub_2. eauto.
+  - intros. pose proof esub_is_term_erased_cosub_1. eauto.
+Qed.
+
+(* topLike specification eqv *)
+Definition toplikeSpec A := esub typ_top A.
+
+Theorem ord_or_spl : forall A,
+    ord A \/ exists B C, spl A B C.
+Proof.
+  introv. induction* A.
+  - inverts* IHA2.
+  - inverts* IHA.
+Qed.
+
+Theorem toplike_spl : forall A B C,
+    toplike A -> spl A B C -> toplike B /\ toplike C.
+Proof.
+  intros. gen B C. induction* H; intros; try solve_by_invert.
+  - inverts* H1.
+  - inverts* H0. forwards*: IHtoplike H5.
+  - inverts* H0. forwards*: IHtoplike H5.
+Qed.
+
+
+Theorem toplike_spl_2 : forall A B C,
+    spl A B C -> toplike B -> toplike C -> toplike A.
+Proof.
+  introv HS HT1 HT2. induction* HS.
+  all: inverts HT1; inverts* HT2.
+Qed.
+
+Theorem toplike_spec_sound_and_complete: forall A,
+    toplike A <-> toplikeSpec A.
+Proof with try solve_by_invert; eauto.
+  unfold toplikeSpec; split; intros.
+  - indTypSize (size_typ A).
+    forwards* [?| (?&?&?) ]: ord_or_spl A.
+    forwards~ (?&?): toplike_spl H0.
+    applys ES_Split H0; applys~ IH; elia.
+  - indTypSize (size_typ A).
+    inverts* H.
+    forwards: IH H1. elia. forwards: IH H2. elia.
+    eauto using toplike_spl_2.
+Qed.
+
+Corollary super_top_toplike : forall A,
+    esub typ_top A -> toplike A.
+Proof.
+  intros. apply toplike_spec_sound_and_complete.
+  eauto.
+Qed.
+
+Lemma toplike_covariance : forall A B,
+    toplike A -> esub A B -> toplike B.
+Proof with eauto using toplike_spec_sound_and_complete.
+  introv HT HS.
+  induction* HS...
+  all: inverts* HT.
+  all:  applys toplike_spl_2...
+Qed.
+
+Definition disjointSpec A B :=
+  forall C, esub A C -> esub B C -> toplike C.
+
+(* split *)
+Lemma split_ord_false : forall T T1 T2,
+    spl T T1 T2 -> ord T -> False.
+Proof.
+  introv s o. gen T1 T2.
+  induction o; intros; inverts* s.
+Qed.
+
+#[local] Hint Resolve split_ord_false : FalseHd.
+
+Lemma disjoint_rcd: forall A B l,
+    disjoint (typ_rcd l A) (typ_rcd l B) -> disjoint A B.
+Proof.
+  introv H.
+  inverts* H; intuition eauto.
+  all: inverts* H0.
+Qed.
+
+#[export] Hint Immediate disjoint_rcd : core.
+
+Lemma split_unique : forall T A1 A2 B1 B2,
+    spl T A1 B1 -> spl T A2 B2 -> A1 = A2 /\ B1 = B2.
+Proof.
+  introv s1 s2. gen A2 B2.
+  induction s1; intros;
+    inverts* s2;
+    forwards* (eq1&eq2): IHs1; split; congruence.
+Qed.
+
+Ltac split_unify :=
+  repeat match goal with
+    | [ H1: spl ?A _ _ , H2: spl ?A _ _ |- _ ] =>
+        (progress forwards (?&?): split_unique H1 H2;
+         subst; clear H2)
+    | [ H: spl (typ_and _ _) _ _ |- _ ] => inverts H
+    | [ H: spl (typ_arrow _ _) _ _ |- _ ] => inverts H
+    | [ H: spl (typ_rcd _ _) _ _ |- _ ] => inverts H
+    end;
+  auto.
+
+
+Theorem disjoint_soundness: forall A B,
+    disjoint A B -> disjointSpec A B.
+Proof with (solve_false; auto).
+  intros A B Dis C S1 S2.
+  indTypSize (size_typ A + size_typ B + size_typ C).
+
+  forwards [?|(?&?&?)]: ord_or_spl C.
+  - inverts Dis;
+      try solve [applys* toplike_covariance];
+      try solve [inverts S1; inverts S2; solve_false; auto]...
+    + inverts S1...
+      forwards: IH H6 S2; elia...
+      forwards: IH H6 S2; elia...
+    + inverts S2...
+      forwards: IH S1 H6; elia...
+      forwards: IH S1 H6; elia...
+    + inverts S1; inverts S2...
+      apply TL_arr.
+      forwards: IH H0 H7 H12; elia...
+    + inverts S1; inverts S2...
+      apply TL_rcd.
+      forwards: IH H0 H6 H9; elia...
+  -
+    inverts S1; inverts S2...
+    split_unify.
+    applys toplike_spl_2 H; applys* IH Dis; elia.
+Qed.
+
+(* generalize S_top *)
+Lemma toplike_super_any : forall A B,
+    toplike A -> esub B A.
+Proof.
+  introv TL. indTypSize (size_typ A).
+  forwards* [?| (?&?&?) ]: ord_or_spl A.
+  forwards (?&?): toplike_spl TL H.
+  forwards*: IH x; elia.
+  forwards*: IH x0; elia.
+Qed.
+
+(* generalize S_andl *)
+Lemma sub_l_andl : forall A B C, esub A C -> esub (typ_and A B) C.
+Proof.
+  introv s. induction* s.
+Qed.
+
+(* generalize S_andr *)
+Lemma sub_l_andr : forall A B C, esub B C -> esub (typ_and A B) C.
+Proof.
+  introv s. induction* s.
+Qed.
+
+(* generalize S_arr *)
+Lemma sub_fun : forall A B C D,
+    esub B D -> esub C A ->
+    esub (typ_arrow A B) (typ_arrow C D).
+Proof with eauto using toplike_dec.
+  introv s. forwards: toplike_dec D.
+  induction* s...
+  all: destruct* H.
+Qed.
+
+(* generalize S_rcd *)
+Lemma sub_rcd : forall A B l,
+    esub A B -> esub (typ_rcd l A) (typ_rcd l B).
+Proof with eauto using toplike_dec.
+  introv s. forwards: toplike_dec B.
+  induction* s...
+  all: destruct* H.
+Qed.
+
+#[export]
+  Hint Immediate toplike_super_any : core.
+#[export]
+  Hint Resolve sub_l_andl sub_l_andr sub_fun sub_rcd: core.
+
+
+Lemma sub_refl : forall A,
+    esub A A.
+Proof.
+  introv. induction* A.
+  - forwards* [?|?]: toplike_dec typ_bot.
+Qed.
+
+
+Lemma sub_bot : forall A,
+    esub typ_bot A.
+Proof with eauto using toplike_dec.
+  introv. forwards: toplike_dec A.
+  indTypSize (size_typ A).
+  forwards* [?| (?&?&?) ]: ord_or_spl A.
+  all: destruct* H.
+  - forwards: IH x... elia.
+    forwards: IH x0... elia.
+Qed.
+
+#[local] Hint Resolve sub_refl sub_bot : core.
+
+Fixpoint term_eq_dec (l1 l2 : label) : {l1 = l2} + {l1 <> l2}.
+Proof.
+  repeat decide equality.
+Defined.
+
+Theorem disjoint_completeness: forall A B,
+    disjointSpec A B -> disjoint A B.
+Proof.
+  intros A B.
+  unfold disjointSpec.
+  - gen B.
+    induction A;
+      introv H; auto.
+    all: induction B; auto.
+    + (* arr arr *)
+      forwards* [?|?]: toplike_dec A2.
+      forwards* [?|?]: toplike_dec B2.
+      applys* D_ArrArr. applys* IHA2.
+      intros.
+      forwards: H (typ_arrow (typ_and A1 B1) C).
+      1-2: applys* sub_fun.
+      inverts~ H2.
+    + (* rcd rcd *)
+      case_eq (term_eq_dec l l0); intros; auto; subst.
+      apply D_rcdEq. apply IHA. introv s1 s2.
+      assert (TL: toplike (typ_rcd l0 C) ). {
+        apply~ H.
+      }
+      inverts~ TL.
+Qed.
+
 
 Lemma cosub_well_typed : forall E t1 A B t2 At,
     cosub t1 A B t2 -> target_typing E t1 At -> subTarget At |[A]| ->
@@ -274,12 +877,12 @@ intuition eauto using target_typing_wf_1, target_typing_wf_2,
     all: eauto...
   - (* arrow *)
     pick fresh y.
-    lets* (HS1 & HS2): H1 y.
+    lets* (? & HS1 & HS2): H1 y.
 
     lets (?&?&Eq): lookup_ST_sub (|| (typ_arrow A1 A2) ||) ST.
     (* lets* (?&?&?&?&?): flex_typing_property3 (|| (typ_arrow A1 A2) ||) HT. *)
     rewrite ttyp_trans_ord_ntop_arrow. 2: eauto. simpl. case_if...
-    applys check_toplike_false. applys* cosub_not_toplike.
+    applys check_toplike_false_2. applys* cosub_not_toplike.
 
     forwards (?&?&?&?&?&?&?): ST_arrow_inv Eq. subst.
 
@@ -297,15 +900,15 @@ intuition eauto using target_typing_wf_1, target_typing_wf_2,
     auto...
     exists. splits. applys TTyping_RcdCons.
     4: econstructor...
-      3: {
-        pick fresh z and apply TTyping_Abs.
-        forwards* : subst_var_typing H8.
-        solve_notin.
-      }
-      3: eauto.
-      2: right*.
-      1: now eauto.
-      rewrite ttyp_trans_ord_ntop_arrow...
+    3: {
+      pick fresh z and apply TTyping_Abs.
+      forwards* : subst_var_typing H8.
+      solve_notin.
+    }
+    3: eauto.
+    2: right*.
+    1: now eauto.
+    rewrite ttyp_trans_ord_ntop_arrow...
     simpl. case_if*. {
       exfalso. applys H0. rewrite <- check_toplike_sound_complete in C.
       eauto using comerge_toplike_r.
@@ -391,16 +994,16 @@ Lemma distapp_well_typed_app : forall A B C G t1 t2 t3 A' B',
     target_typing ||[ G ]|| t2 B' -> subTarget B' |[B]| ->
     exists C', target_typing ||[ G ]|| t3 C' /\ subTarget C' |[C]| /\ subTarget |[C]| C'.
 Proof with intuition eauto using target_typing_wf_1, target_typing_wf_2,
-  target_typing_wf_typ, ST_refl, ST_trans, ST_toplike, ST_top, ST_rcd_2,
-  cosub_not_toplike, ttyp_trans_wf,
-  translate_to_record_types, subTarget_rec_typ.
+    target_typing_wf_typ, ST_refl, ST_trans, ST_toplike, ST_top, ST_rcd_2,
+    cosub_not_toplike, ttyp_trans_wf,
+    translate_to_record_types, subTarget_rec_typ.
 
   introv HA HTa HEa HTb HEb. gen A' B'.
   inductions HA; intros.
   - rewrite* ttyp_trans_ord_top.
   - forwards* (?&?&?): cosub_well_typed H1.
     lets (?&?&?&?): lookup_ST_sub (|| (typ_arrow A B) ||) HEa.
-     simpl. case_if*.
+    simpl. case_if*.
     { apply check_toplike_sound_complete in C0. contradiction. }
     forwards(?&?&?&?&?&?&?): ST_arrow_inv H5. subst.
     exists. splits. applys TTyping_App.
@@ -408,8 +1011,8 @@ Proof with intuition eauto using target_typing_wf_1, target_typing_wf_2,
   - forwards* (?&?&?&?): IHHA1 HTb. eauto using ST_refl, ST_trans, ST_andl.
     forwards* (?&?&?&?): IHHA2 HTb. eauto using ST_refl, ST_trans, ST_andr.
     forwards*: concat_source_intersection...
-    forwards* (?&?&?&?): ST_concat H5 H1 H3...
-    exists. split. applys* TTyping_RcdMerge H H2.
+    forwards* (?&?&?&?): ST_concat H6 H1 H4...
+    exists. split. applys* TTyping_RcdMerge H0 H3.
     all: eauto...
 Qed.
 
@@ -419,8 +1022,8 @@ Lemma distapp_well_typed_proj : forall A l t1 t3 C G A',
     subTarget A' |[A]| ->
     exists C', target_typing ||[ G ]|| t3 C' /\ subTarget C' |[C]| /\ subTarget |[C]| C'.
 Proof with intuition eauto using target_typing_wf_1, target_typing_wf_2,
-  target_typing_wf_typ, ST_refl, ST_trans, ST_toplike, ST_top, ST_rcd_2,
-  cosub_not_toplike,
+    target_typing_wf_typ, ST_refl, ST_trans, ST_toplike, ST_top, ST_rcd_2,
+    cosub_not_toplike,
     translate_to_record_types, subTarget_rec_typ.
 
   introv HA HT HS. gen A'.
@@ -434,8 +1037,8 @@ Proof with intuition eauto using target_typing_wf_1, target_typing_wf_2,
   - forwards* (?&?&?): IHHA1 HT; eauto using ST_refl, ST_trans, ST_andl.
     forwards* (?&?&?): IHHA2 HT; eauto using ST_refl, ST_trans, ST_andr.
     forwards*: concat_source_intersection...
-    forwards* (?&?&?&?): ST_concat H3 H4 H0...
-    exists. split. applys* TTyping_RcdMerge H H1.
+    forwards* (?&?&?&?): ST_concat H4 H5 H1...
+    exists. split. applys* TTyping_RcdMerge H0 H2.
     all: eauto...
 Qed.
 
@@ -443,8 +1046,8 @@ Theorem elaboration_well_typed : forall G e dirflag A t,
     elaboration G e dirflag A t ->
     exists A', target_typing ||[ G ]|| t A' /\  subTarget A' |[A]| /\  subTarget |[A]| A'.
 Proof with intuition eauto using target_typing_wf_1, target_typing_wf_2,
-  target_typing_wf_typ, ST_refl, ST_trans, ST_toplike, ST_top, ST_rcd_2,
-  cosub_not_toplike, ctx_trans_preserves_uniq, ttyp_trans_wf,
+    target_typing_wf_typ, ST_refl, ST_trans, ST_toplike, ST_top, ST_rcd_2,
+    cosub_not_toplike, ctx_trans_preserves_uniq, ttyp_trans_wf,
     translate_to_record_types, subTarget_rec_typ,  elaboration_wf_ctx.
   introv HT.
   induction HT...
